Fp/Theorems/AgainstSMT.lean
@@ -6,38 +6,38 @@ def twoE3M4 : PackedFloat 3 4 := PackedFloat.ofBits 3 4 0b01000000#8
 def oneE3M4 : PackedFloat 3 4 := PackedFloat.ofBits 3 4 0b00110000#8
 
 theorem add_comm (a b : PackedFloat 3 4)
-  : (add a b .RNE) = (add b a .RNE) := by
+  : (a + b) = (b + a) := by
   bv_decide
 
 theorem add_monotone (a b c : PackedFloat 3 4) (hc : c.isNormOrSubnorm)
-  : le a b → le (add a c .RNE) (add b c .RNE) := by
+  : PackedFloat.smtBle a b → PackedFloat.smtBle (a + c) (b + c) := by
   bv_decide
 
 theorem add_eq_mul_two (a : PackedFloat 3 4)
-  : add a a .RNE = mul twoE3M4 a .RNE := by
+  : a + a = twoE3M4 * a := by
   bv_decide
 
 theorem mul_comm (a b : PackedFloat 3 4)
-  : (mul a b .RNE) = (mul b a .RNE) := by
+  : a * b = b * a := by
   bv_decide
 
 theorem mul_one_is_id (a : PackedFloat 3 4)
   (h : ¬a.isNaN)
-  : eq (mul a oneE3M4 .RNE) a := by
+  : a * oneE3M4 = a := by
   bv_decide
 
 theorem div_one_is_id (a : PackedFloat 3 4)
   (h : ¬a.isNaN)
-  : eq (div a oneE3M4 .RNE) a := by
+  : a / oneE3M4 = a := by
   bv_decide
 
 theorem div_self_is_one (a : PackedFloat 3 4)
   (h : ¬a.isNaN ∧ ¬a.isInfinite ∧ ¬a.isZero)
-  : (div a a .RNE) = oneE3M4 := by
+  : a / a = oneE3M4 := by
   bv_decide
 
 theorem rem_lt_abs_self (a b : PackedFloat 3 4)
   (h : a.isNormOrSubnorm)
   (hb : ¬b.isNaN ∧ ¬b.isZero)
-  : lt (remainder a b) (abs b) := by
+  : PackedFloat.smtBlt (remainder a b) (b.abs) := by
   bv_decide
